move phase two to its own file, define merge point

systems/ChordCorrectness.v
@@ -22,99 +22,10 @@ Require Import Chord.ChordPromises.
 Require Import Chord.ChordDefinitionLemmas.
 Require Import Chord.ChordLocalProps.
 Require Import Chord.ChordPhaseOne.
+Require Import Chord.ChordPhaseTwo.
 
 Set Bullet Behavior "Strict Subproofs".
 Open Scope nat_scope.
-
-Definition live_addrs (gst : global_state) : list addr :=
-  filter (fun a => Coqlib.proj_sumbool (live_node_dec gst a))
-         (nodes gst).
-
-Definition live_ptrs (gst : global_state) : list pointer :=
-  map make_pointer (live_addrs gst).
-
-Definition live_ptrs_with_states (gst : global_state) : list (pointer * data) :=
-  FilterMap.filterMap (fun p =>
-                         match sigma gst (addr_of p) with
-                         | Some st => Some (p, st)
-                         | None => None
-                         end)
-                      (live_ptrs gst).
-
-Definition full_succs (gst : global_state) (h : pointer) (succs : list pointer) : Prop :=
-  length succs = Chord.SUCC_LIST_LEN.
-
-Lemma successor_nodes_valid_state :
-  forall gst h p st,
-    In p (succ_list st) ->
-    successor_nodes_valid gst ->
-    sigma gst h = Some st ->
-    exists pst, sigma gst (addr_of p) = Some pst /\
-           joined pst = true.
-Proof.
-  intros.
-  eapply_prop_hyp successor_nodes_valid @eq; eauto.
-  now break_and.
-Qed.
-
-Lemma nonempty_succ_lists_always_belong_to_joined_nodes :
-  forall gst h st,
-    reachable_st gst ->
-    sigma gst h = Some st ->
-    succ_list st <> [] ->
-    joined st = true.
-Proof.
-Admitted.
-
-Lemma zero_leading_failed_nodes_leading_node_live :
-  forall gst h st s rest,
-    succ_list_leading_failed_nodes (failed_nodes gst) (succ_list st) = 0 ->
-    reachable_st gst ->
-    sigma gst h = Some st ->
-    succ_list st = s :: rest ->
-    wf_ptr s ->
-    wf_ptr s /\ live_node gst (addr_of s).
-Proof.
-  intros.
-  repeat find_rewrite.
-  simpl in *.
-  break_if; try congruence.
-  unfold succ_list_leading_failed_nodes.
-  find_apply_lem_hyp successor_nodes_always_valid.
-  assert (In s (succ_list st)).
-  {
-    find_rewrite.
-    apply in_eq.
-  }
-  find_eapply_lem_hyp successor_nodes_valid_inv; eauto; repeat (break_exists_name pst || break_and).
-  eauto using live_node_characterization.
-Qed.
-
-Lemma live_node_has_Tick_in_timeouts :
-  forall ex h,
-    lb_execution ex ->
-    reachable_st (occ_gst (hd ex)) ->
-    live_node (occ_gst (hd ex)) h ->
-    In Tick (timeouts (occ_gst (hd ex)) h).
-Admitted.
-
-Lemma loaded_Tick_enabled_if_now_not_busy_if_live :
-  forall h ex,
-    lb_execution ex ->
-    reachable_st (occ_gst (hd ex)) ->
-    strong_local_fairness ex ->
-    live_node (occ_gst (hd ex)) h ->
-    now (not_busy_if_live h) ex ->
-    now (l_enabled (Timeout h Tick StartStabilize)) ex.
-Proof.
-  intros.
-  destruct ex.
-  find_copy_apply_lem_hyp live_node_has_Tick_in_timeouts; eauto.
-  simpl in *.
-  find_copy_apply_lem_hyp live_node_joined; break_exists; break_and.
-  unfold not_busy_if_live in *; find_copy_apply_hyp_hyp.
-  eapply loaded_Tick_enabled_when_cur_request_None; eauto.
-Qed.
 
 (* this isn't used anywhere but might be useful in the future *)
 Lemma request_always_effective :
@@ -148,112 +59,6 @@ Proof.
   unfold recv_handler_l.
   congruence.
 Qed.
-
-(** In phase two we want to talk about the existence and number of better
-    predecessors and better first successors to a node. We do this with the
-    following functions.
-    - better_* : Prop, which holds if a node is closer to h.
-    - better_*_bool : bool, which is true if some live node is a better pointer for h.
-    - *_correct : Prop, which holds if the pointer is globally correct.
-    - *_error : nat, which counts the number of better options for the pointer.
-    We prove that error = 0 <-> correct so we can use an argument about the
-    measure to prove eventual correctness.
- *)
-
-Definition counting_opt_error (gst : global_state) (p : option pointer) (better_bool : pointer -> pointer -> bool) : nat :=
-  match p with
-  | Some p0 =>
-    if live_node_dec gst (addr_of p0)
-    then length (filter (better_bool p0) (live_ptrs gst))
-    else length (live_ptrs gst) + 1
-  | None => length (live_ptrs gst) + 1
-  end.
-
-Lemma counting_opt_error_zero_implies_correct :
-  forall gst p better_bool,
-    counting_opt_error gst p better_bool = 0 ->
-    exists p0,
-      p = Some p0 /\
-      forall p',
-        live_node gst (addr_of p') ->
-        wf_ptr p' ->
-        better_bool p0 p' = false.
-Proof.
-  unfold counting_opt_error.
-  intros.
-  repeat break_match.
-Admitted.
-
-(** Predecessor phase two definitions *)
-Definition better_pred (gst : global_state) (h p p' : pointer) : Prop :=
-  wf_ptr p /\
-  wf_ptr p' /\
-  live_node gst (addr_of p') /\
-  ptr_between p p' h.
-
-Definition better_pred_bool (h p p' : pointer) : bool :=
-  ptr_between_bool p p' h.
-
-Definition pred_correct (gst : global_state) (h : pointer) (p : option pointer) : Prop :=
-  exists p0,
-    p = Some p0 /\
-    forall p',
-      ~ better_pred gst h p0 p'.
-
-Definition pred_error (gst : global_state) (h : pointer) (p : option pointer) : nat :=
-  counting_opt_error gst p (better_pred_bool h).
-
-(** First successor phase two definitions *)
-Definition better_succ (gst : global_state) (h s s' : pointer) : Prop :=
-  wf_ptr s /\
-  wf_ptr s' /\
-  live_node gst (addr_of s') /\
-  ptr_between h s' s.
-
-Definition better_succ_bool (h s s' : pointer) : bool :=
-  ptr_between_bool h s' s.
-
-Definition first_succ_correct (gst : global_state) (h : pointer) (p : option pointer) : Prop :=
-  exists p0,
-    p = Some p0 /\
-    forall p', ~ better_succ gst h p0 p'.
-
-Definition first_succ_error (gst : global_state) (h : pointer) (s : option pointer) : nat :=
-  counting_opt_error gst s (better_succ_bool h).
-
-(** First successor and predecessor combined phase two definitions *)
-Definition pred_and_first_succ_correct (gst : global_state) (h : pointer) (st : data) : Prop :=
-  pred_correct gst h (pred st) /\
-  first_succ_correct gst h (hd_error (succ_list st)).
-
-Definition pred_and_first_succ_error (h : addr) (gst : global_state) : nat :=
-  match sigma gst h with
-  | Some st =>
-    pred_error gst (make_pointer h) (pred st) +
-    first_succ_error gst (make_pointer h) (hd_error (succ_list st))
-  | None =>
-    length (active_nodes gst) + 1
-  end.
-
-Definition phase_two_error : global_state -> nat :=
-  global_measure pred_and_first_succ_error.
-
-Definition preds_and_first_succs_correct (gst : global_state) : Prop :=
-  forall h st,
-    live_node gst (addr_of h) ->
-    wf_ptr h ->
-    sigma gst (addr_of h) = Some st ->
-    pred_and_first_succ_correct gst h st.
-
-Lemma phase_two_zero_error_locally_correct :
-  forall gst h st,
-    live_node gst (addr_of h) ->
-    wf_ptr h ->
-    sigma gst (addr_of h) = Some st ->
-    pred_and_first_succ_error (addr_of h) gst = 0 ->
-    pred_and_first_succ_correct gst h st.
-Proof.
-Admitted.
 
 Lemma live_addr_In_live_addrs :
   forall gst h,
@@ -292,56 +97,6 @@ Proof.
   apply FilterMap.filterMap_In with (a:=h).
   - by find_rewrite.
   - by apply live_In_live_ptrs.
-Qed.
-
-Lemma phase_two_zero_error_correct :
-  forall gst,
-    phase_two_error gst = 0 ->
-    preds_and_first_succs_correct gst.
-Proof.
-Admitted.
-
-(* This is really an invariant. *)
-Lemma phase_two_error_stable :
-  forall ex,
-    lb_execution ex ->
-    reachable_st (occ_gst (hd ex)) ->
-    continuously
-      (consecutive
-         (measure_nonincreasing phase_two_error))
-      ex.
-Proof.
-Admitted.
-
-(* This is the hard part. *)
-Lemma phase_two_error_decreasing :
-  forall ex,
-    lb_execution ex ->
-    reachable_st (occ_gst (hd ex)) ->
-    strong_local_fairness ex ->
-    always (~_ (now circular_wait)) ex ->
-    always (zero_or_eventually_decreasing phase_two_error) ex.
-Proof.
-Admitted.
-
-Lemma phase_two :
-  forall ex,
-    lb_execution ex ->
-    reachable_st (occ_gst (hd ex)) ->
-    strong_local_fairness ex ->
-    always (~_ (now circular_wait)) ex ->
-    continuously (lift_gpred_to_ex preds_and_first_succs_correct) ex.
-Proof.
-  intros.
-  find_copy_apply_lem_hyp phase_two_error_stable; auto.
-  find_copy_apply_lem_hyp phase_two_error_decreasing; auto.
-  find_copy_apply_lem_hyp measure_decreasing_to_zero_continuously; auto.
-  unfold lift_gpred_to_ex.
-  eapply continuously_monotonic.
-  - eapply now_monotonic; intros.
-    apply phase_two_zero_error_correct.
-    eauto using measure_zero_elim.
-  - assumption.
 Qed.
 
 (** Phase three: all successors become correct. *)
@@ -460,6 +215,24 @@ Proof.
   now auto using phases_locally_sufficient.
 Qed.
 
+Lemma phase_two_without_phase_one :
+  forall ex : infseq occurrence,
+    lb_execution ex ->
+    reachable_st (occ_gst (hd ex)) ->
+    strong_local_fairness ex ->
+    always (~_ now circular_wait) ex ->
+    continuously (now phase_two) ex.
+Proof.
+  intros.
+  find_copy_eapply_lem_hyp phase_one_continuously; eauto.
+  apply eventually_idempotent.
+  lift_eventually phase_two_continuously.
+  - intros.
+    unfold and_tl in *; break_and.
+    repeat (split; invar_eauto).
+  - firstorder.
+Qed.
+
 Theorem chord_stabilization :
   forall ex : infseq.infseq occurrence,
     reachable_st (occ_gst (infseq.hd ex)) ->
@@ -471,7 +244,7 @@ Theorem chord_stabilization :
       ex.
 Proof.
   intros.
-  find_copy_eapply_lem_hyp phase_two; eauto.
+  find_copy_eapply_lem_hyp phase_two_without_phase_one; eauto.
   find_copy_eapply_lem_hyp phase_three; eauto.
   eapply continuously_monotonic.
   eapply phases_sufficient.
@@ -479,5 +252,5 @@ Proof.
   - intros.
     rewrite and_tl_gpred_and_comm.
     eauto.
-  - now apply continuously_and_tl.
+  - apply continuously_and_tl; eauto.
 Qed.
