systems/ChordPhaseTwo.v
@@ -1,0 +1,321 @@
+Require Import List.
+Import ListNotations.
+Require Import Omega.
+
+Require Verdi.Coqlib.
+Require Import StructTact.StructTactics.
+Require Import StructTact.Update.
+Require Import InfSeqExt.infseq.
+Require Import Chord.InfSeqTactics.
+Require Import Chord.Measure.
+
+Require Import Chord.Chord.
+Import Chord.Chord.Chord.
+Import ChordIDSpace.
+Require Import Chord.ChordProof.
+Require Import Chord.ChordSemantics.
+Import ChordSemantics.
+Import ConstrainedChord.
+Require Import Chord.ChordValidPointersInvariant.
+Require Import Chord.ChordLabeled.
+Require Import Chord.ChordPromises.
+Require Import Chord.ChordDefinitionLemmas.
+Require Import Chord.ChordLocalProps.
+Require Import Chord.ChordPhaseOne.
+
+Set Bullet Behavior "Strict Subproofs".
+Open Scope nat_scope.
+
+Definition live_addrs (gst : global_state) : list addr :=
+  filter (fun a => Coqlib.proj_sumbool (live_node_dec gst a))
+         (nodes gst).
+
+Definition live_ptrs (gst : global_state) : list pointer :=
+  map make_pointer (live_addrs gst).
+
+Definition live_ptrs_with_states (gst : global_state) : list (pointer * data) :=
+  FilterMap.filterMap (fun p =>
+                         match sigma gst (addr_of p) with
+                         | Some st => Some (p, st)
+                         | None => None
+                         end)
+                      (live_ptrs gst).
+
+Definition full_succs (gst : global_state) (h : pointer) (succs : list pointer) : Prop :=
+  length succs = Chord.SUCC_LIST_LEN.
+
+Lemma successor_nodes_valid_state :
+  forall gst h p st,
+    In p (succ_list st) ->
+    successor_nodes_valid gst ->
+    sigma gst h = Some st ->
+    exists pst, sigma gst (addr_of p) = Some pst /\
+           joined pst = true.
+Proof.
+  intros.
+  eapply_prop_hyp successor_nodes_valid @eq; eauto.
+  now break_and.
+Qed.
+
+Lemma nonempty_succ_lists_always_belong_to_joined_nodes :
+  forall gst h st,
+    reachable_st gst ->
+    sigma gst h = Some st ->
+    succ_list st <> [] ->
+    joined st = true.
+Proof.
+Admitted.
+
+Lemma zero_leading_failed_nodes_leading_node_live :
+  forall gst h st s rest,
+    succ_list_leading_failed_nodes (failed_nodes gst) (succ_list st) = 0 ->
+    reachable_st gst ->
+    sigma gst h = Some st ->
+    succ_list st = s :: rest ->
+    wf_ptr s ->
+    wf_ptr s /\ live_node gst (addr_of s).
+Proof.
+  intros.
+  repeat find_rewrite.
+  simpl in *.
+  break_if; try congruence.
+  unfold succ_list_leading_failed_nodes.
+  find_apply_lem_hyp successor_nodes_always_valid.
+  assert (In s (succ_list st)).
+  {
+    find_rewrite.
+    apply in_eq.
+  }
+  find_eapply_lem_hyp successor_nodes_valid_inv; eauto; repeat (break_exists_name pst || break_and).
+  eauto using live_node_characterization.
+Qed.
+
+Lemma live_node_has_Tick_in_timeouts :
+  forall ex h,
+    lb_execution ex ->
+    reachable_st (occ_gst (hd ex)) ->
+    live_node (occ_gst (hd ex)) h ->
+    In Tick (timeouts (occ_gst (hd ex)) h).
+Proof.
+Admitted.
+
+Lemma loaded_Tick_enabled_if_now_not_busy_if_live :
+  forall h ex,
+    lb_execution ex ->
+    reachable_st (occ_gst (hd ex)) ->
+    strong_local_fairness ex ->
+    live_node (occ_gst (hd ex)) h ->
+    now (not_busy_if_live h) ex ->
+    now (l_enabled (Timeout h Tick StartStabilize)) ex.
+Proof.
+  intros.
+  destruct ex.
+  find_copy_apply_lem_hyp live_node_has_Tick_in_timeouts; eauto.
+  simpl in *.
+  find_copy_apply_lem_hyp live_node_joined; break_exists; break_and.
+  unfold not_busy_if_live in *; find_copy_apply_hyp_hyp.
+  eapply loaded_Tick_enabled_when_cur_request_None; eauto.
+Qed.
+
+(** In phase two we want to talk about the existence and number of better
+    predecessors and better first successors to a node. We do this with the
+    following functions.
+    - better_* : Prop, which holds if a node is closer to h.
+    - better_*_bool : bool, which is true if some live node is a better pointer for h.
+    - *_correct : Prop, which holds if the pointer is globally correct.
+    - *_error : nat, which counts the number of better options for the pointer.
+    We prove that error = 0 <-> correct so we can use an argument about the
+    measure to prove eventual correctness.
+ *)
+Definition counting_opt_error (gst : global_state) (p : option pointer) (better_bool : pointer -> pointer -> bool) : nat :=
+  match p with
+  | Some p0 =>
+    if live_node_dec gst (addr_of p0)
+    then length (filter (better_bool p0) (live_ptrs gst))
+    else length (live_ptrs gst) + 1
+  | None => length (live_ptrs gst) + 1
+  end.
+
+Lemma counting_opt_error_zero_implies_correct :
+  forall gst p better_bool,
+    counting_opt_error gst p better_bool = 0 ->
+    exists p0,
+      p = Some p0 /\
+      forall p',
+        live_node gst (addr_of p') ->
+        wf_ptr p' ->
+        better_bool p0 p' = false.
+Proof.
+  unfold counting_opt_error.
+  intros.
+  repeat break_match.
+Admitted.
+
+(** Predecessor phase two definitions *)
+Definition better_pred (gst : global_state) (h p p' : pointer) : Prop :=
+  wf_ptr p /\
+  wf_ptr p' /\
+  live_node gst (addr_of p') /\
+  ptr_between p p' h.
+
+Definition better_pred_bool (h p p' : pointer) : bool :=
+  ptr_between_bool p p' h.
+
+Definition pred_correct (gst : global_state) (h : pointer) (p : option pointer) : Prop :=
+  exists p0,
+    p = Some p0 /\
+    forall p',
+      ~ better_pred gst h p0 p'.
+
+Definition pred_error (gst : global_state) (h : pointer) (p : option pointer) : nat :=
+  counting_opt_error gst p (better_pred_bool h).
+
+(** First successor phase two definitions *)
+Definition better_succ (gst : global_state) (h s s' : pointer) : Prop :=
+  wf_ptr s /\
+  wf_ptr s' /\
+  live_node gst (addr_of s') /\
+  ptr_between h s' s.
+
+Definition better_succ_bool (h s s' : pointer) : bool :=
+  ptr_between_bool h s' s.
+
+Definition first_succ_correct (gst : global_state) (h : pointer) (p : option pointer) : Prop :=
+  exists p0,
+    p = Some p0 /\
+    forall p', ~ better_succ gst h p0 p'.
+
+Definition first_succ_error (gst : global_state) (h : pointer) (s : option pointer) : nat :=
+  counting_opt_error gst s (better_succ_bool h).
+
+(** First successor and predecessor combined phase two definitions *)
+Definition pred_and_first_succ_correct (gst : global_state) (h : pointer) (st : data) : Prop :=
+  pred_correct gst h (pred st) /\
+  first_succ_correct gst h (hd_error (succ_list st)).
+
+Definition pred_and_first_succ_error (h : addr) (gst : global_state) : nat :=
+  match sigma gst h with
+  | Some st =>
+    pred_error gst (make_pointer h) (pred st) +
+    first_succ_error gst (make_pointer h) (hd_error (succ_list st))
+  | None =>
+    length (active_nodes gst) + 1
+  end.
+
+Definition phase_two_error : global_state -> nat :=
+  global_measure pred_and_first_succ_error.
+
+Definition preds_and_first_succs_correct (gst : global_state) : Prop :=
+  forall h st,
+    live_node gst (addr_of h) ->
+    sigma gst (addr_of h) = Some st ->
+    wf_ptr h ->
+    pred_and_first_succ_correct gst h st.
+
+Definition phase_two (o : occurrence) : Prop :=
+  preds_and_first_succs_correct (occ_gst o).
+
+Lemma phase_two_zero_error_locally_correct :
+  forall gst h st,
+    live_node gst (addr_of h) ->
+    wf_ptr h ->
+    sigma gst (addr_of h) = Some st ->
+    pred_and_first_succ_error (addr_of h) gst = 0 ->
+    pred_and_first_succ_correct gst h st.
+Proof.
+Admitted.
+
+Lemma phase_two_zero_error_correct :
+  forall gst,
+    phase_two_error gst = 0 ->
+    preds_and_first_succs_correct gst.
+Proof.
+Admitted.
+
+Definition has_pred (gst : global_state) (h : pointer) (p : option pointer) : Prop :=
+  exists st,
+    sigma gst (addr_of h) = Some st /\
+    pred st = p.
+
+Definition has_first_succ (gst : global_state) (h s : pointer) : Prop :=
+  exists st,
+    sigma gst (addr_of h) = Some st /\
+    hd_error (succ_list st) = Some s.
+
+Definition merge_point (gst : global_state) (a b j : pointer) : Prop :=
+  ptr_between a b j /\
+  has_first_succ gst a j /\
+  has_first_succ gst b j /\
+  wf_ptr a /\
+  wf_ptr b /\
+  wf_ptr j /\
+  live_node gst (addr_of a) /\
+  live_node gst (addr_of b) /\
+  live_node gst (addr_of j).
+
+Definition pred_or_succ_improves (h : pointer) : infseq occurrence -> Prop :=
+  consecutive (measure_decreasing (pred_and_first_succ_error (addr_of h))).
+
+Lemma error_decreases_at_merge_point :
+  forall ex,
+    lb_execution ex ->
+    reachable_st (occ_gst (hd ex)) ->
+    strong_local_fairness ex ->
+    always (~_ (now circular_wait)) ex ->
+    always (now phase_one) ex ->
+
+    forall a b j,
+      merge_point (occ_gst (hd ex)) a b j ->
+      eventually (pred_or_succ_improves a) ex \/
+      eventually (pred_or_succ_improves b) ex \/
+      eventually (pred_or_succ_improves j) ex.
+Proof.
+Admitted.
+
+Theorem phase_two_error_continuously_nonincreasing :
+  forall ex,
+    lb_execution ex ->
+    reachable_st (occ_gst (infseq.hd ex)) ->
+    strong_local_fairness ex ->
+    always (~_ (now circular_wait)) ex ->
+    always (now phase_one) ex ->
+    continuously (local_measures_nonincreasing pred_and_first_succ_error) ex.
+Proof.
+Admitted.
+
+Lemma continuously_zero_phase_two_error_phase_two :
+  forall ex,
+    lb_execution ex ->
+    reachable_st (occ_gst (hd ex)) ->
+    continuously (now (measure_zero phase_two_error)) ex ->
+    continuously (now phase_two) ex.
+Proof.
+Admitted.
+
+Lemma phase_two_nonzero_error_causes_measure_drop :
+  forall ex : infseq occurrence,
+    lb_execution ex ->
+    reachable_st (occ_gst (hd ex)) ->
+    strong_local_fairness ex ->
+    always (~_ now circular_wait) ex ->
+    always (now phase_one) ex ->
+    continuously (nonzero_error_causes_measure_drop pred_and_first_succ_error) ex.
+Proof.
+  (* Use some lemma about merge points *)
+Admitted.
+
+Lemma phase_two_continuously :
+  forall ex,
+    lb_execution ex ->
+    reachable_st (occ_gst (hd ex)) ->
+    strong_local_fairness ex ->
+    always (~_ (now circular_wait)) ex ->
+    always (now phase_one) ex ->
+    continuously (now phase_two) ex.
+Proof.
+  intros.
+  eapply continuously_zero_phase_two_error_phase_two; eauto.
+  eapply local_measure_causes_measure_zero_continuosly; eauto.
+  - eapply phase_two_error_continuously_nonincreasing; eauto.
+  - eapply phase_two_nonzero_error_causes_measure_drop; eauto.
+Qed.
